1) reproved DSE with the low-level memory simulation that SAS uses.
The proof structures of DSE and SAS are very similar, should be able to
merge into a more general proof.

2) proved a new property for promotable locations: if a block b is
promotable for a alloca with type t, the memory range of b must contain
[0, size of t). This property was used by DSE. 

Consider the program state that returns from a call, and inside the call there 
is a promotable location at b. In the call, the simulation ignores
b.[0, size of t). When the call is returned, the simulation does not ignore 
b.[0, size of t) because the promotable alloca does not exist in the current 
stack frames. This is fine because that alloca at b was already deallocated, 
and never accessible. With the proved property, we know that the
allocated range of b contains the memory range the simulation ignored.



git-svn-id: https://webdav.seas.upenn.edu/svn/sol/vol@3857 eef5ea85-cc2e-0410-bd84-0fae1f012da8

src3.0/Transforms/dse.v
@@ -12,6 +12,7 @@ Require Import palloca_props.
 Require Import mem2reg.
 Require Import memory_props.
 Require Import program_sim.
+Require Import sas_msim.
 Require Import trans_tactic.
 
 Definition fdef_simulation (pinfo: PhiInfo) f1 f2 : Prop :=
@@ -73,24 +74,35 @@ match ECs1, ECs2 with
 | _, _ => False
 end.
 
-Definition no_alias_head_in_tail (pinfo:PhiInfo) ptr
+Definition no_alias_head_in_tail (pinfo:PhiInfo) omb
   (ec0:@Opsem.ExecutionContext DGVs) : Prop :=
-forall gvsa (Heq: Opsem.CurFunction ec0 = PI_f pinfo)
-  (Hlkup: lookupAL _ (Opsem.Locals ec0) (PI_id pinfo) = Some gvsa),
-  MemProps.no_alias ptr gvsa.
+(Opsem.CurFunction ec0 = PI_f pinfo ->
+match lookupAL _ (Opsem.Locals ec0) (PI_id pinfo) with
+| Some ((Vptr mb _, _)::nil) => omb = Some mb
+| _ => omb = None
+end) /\
+(Opsem.CurFunction ec0 <> PI_f pinfo -> omb = None).
 
-Definition no_alias_head_tail (pinfo:PhiInfo) ptr
+Definition no_alias_head_tail (pinfo:PhiInfo) ombs
   (ecs':list Opsem.ExecutionContext) : Prop :=
-  forall ec0 (Hin: In ec0 ecs'), no_alias_head_in_tail pinfo ptr ec0.
+List.Forall2 (fun ec omb => 
+              no_alias_head_in_tail pinfo omb ec) ecs' ombs.
 
-Definition Mem_simulation (pinfo:PhiInfo) TD (ecs1:list Opsem.ExecutionContext)
-  Mem1 Mem2 : Prop :=
+Definition dse_mem_inj (pinfo:PhiInfo) (ecs1:list Opsem.ExecutionContext) 
+  TD (m1 m2: mem) : Prop :=
+match getTypeStoreSize TD (PI_typ pinfo) with
+| Some tsz => 
+    forall ombs,
+      no_alias_head_tail pinfo ombs ecs1 ->
+      SASmsim.mem_inj inject_id (ombs__ignores (Size.to_Z tsz) ombs) m1 m2
+| None => False
+end.
+
+Definition mem_simulation (pinfo:PhiInfo) TD
+  (ecs1:list Opsem.ExecutionContext) Mem1 Mem2 : Prop :=
 Mem.nextblock Mem1 = Mem.nextblock Mem2 /\
-forall ptr ty al gvs1 gvs2
-  (Hnalias: no_alias_head_tail pinfo ptr ecs1)
-  (Hld1: mload TD Mem1 ptr ty al = Some gvs1)
-  (Hld2: mload TD Mem2 ptr ty al = Some gvs2),
-  gvs1 = gvs2.
+(forall b, Mem.bounds Mem1 b = Mem.bounds Mem2 b) /\
+dse_mem_inj pinfo ecs1 TD Mem1 Mem2.
 
 Definition State_simulation (pinfo: PhiInfo)
   (Cfg1:OpsemAux.Config) (St1:Opsem.State)
@@ -102,7 +114,7 @@ match (St1, St2) with
     TD1 = TD2 /\
     products_simulation pinfo Ps1 Ps2 /\
     ECs_simulation pinfo ECs1 ECs2 /\
-    gl1 = gl2 /\ fs1 = fs2 /\ Mem_simulation pinfo TD1 ECs1 M1 M2
+    gl1 = gl2 /\ fs1 = fs2 /\ mem_simulation pinfo TD1 ECs1 M1 M2
 end.
 
 Definition removable_State (pinfo: PhiInfo) (St:@Opsem.State DGVs) : Prop :=
@@ -144,8 +156,8 @@ Proof.
 Qed.
 
 Lemma no_alias_head_tail_irrel :
-  forall pinfo ptr F B1 cs1 tmn1 lc als1 ECs B2 cs2 tmn2 als2,
-  no_alias_head_tail pinfo ptr
+  forall pinfo omb F B1 cs1 tmn1 lc als1 ECs B2 cs2 tmn2 als2,
+  no_alias_head_tail pinfo omb
               ({|
                Opsem.CurFunction := F;
                Opsem.CurBB := B1;
@@ -153,7 +165,7 @@ Lemma no_alias_head_tail_irrel :
                Opsem.Terminator := tmn1;
                Opsem.Locals := lc;
                Opsem.Allocas := als1 |} :: ECs) ->
-  no_alias_head_tail pinfo ptr
+  no_alias_head_tail pinfo omb
               ({|
                Opsem.CurFunction := F;
                Opsem.CurBB := B2;
@@ -163,17 +175,7 @@ Lemma no_alias_head_tail_irrel :
                Opsem.Allocas := als2 |} :: ECs).
 Proof.
   unfold no_alias_head_tail. simpl in *.
-  intros.
-  intros.
-  destruct Hin as [Hin | Hin]; subst; eauto.
-  assert (no_alias_head_in_tail pinfo ptr
-           {| Opsem.CurFunction := F;
-              Opsem.CurBB := B1;
-              Opsem.CurCmds := cs1;
-              Opsem.Terminator := tmn1;
-              Opsem.Locals := lc;
-              Opsem.Allocas := als1 |}) as G. eauto.
-  unfold no_alias_head_in_tail in *. simpl. auto.
+  intros. inv H. constructor; auto.
 Qed.
 
 Lemma cmds_simulation_nil_inv: forall pinfo f1 cs,
@@ -199,7 +201,7 @@ Proof.
   apply H0 in EQ.
   destruct (id_dec (PI_id pinfo) (PI_id pinfo)); simpl in *; congruence.
 Qed.
-
+(*
 Lemma no_alias_head_tail_and_app: forall pinfo ptr ECs1 ECs2,
   no_alias_head_tail pinfo ptr ECs1 ->
   no_alias_head_tail pinfo ptr ECs2 ->
@@ -226,12 +228,6 @@ Proof.
   destruct Hin as [Hin | Hin]; subst; auto.
     inv Hin.
 Qed.
-
-Lemma load_free_allocas_none: forall TD M1 M2 mb als ofs m ty al
-  (Hfree : free_allocas TD M1 als = ret M2)
-  (Hin : In mb als),
-  mload TD M2 ((Vptr mb ofs, m) :: nil) ty al = None.
-Admitted.
 
 Lemma no_alias_head_in_tail__return: forall pinfo F maxb TD M lc als M' EC ptr
   ty al gvs
@@ -260,7 +256,7 @@ Proof.
   erewrite load_free_allocas_none in Hld1'; eauto.
   congruence.
 Qed.
-
+*)
 Ltac destruct_ctx_return :=
 match goal with
 | Hwfcfg : OpsemPP.wf_Config
@@ -342,28 +338,40 @@ Proof.
   destruct (fdef_dec (PI_f pinfo) F); inv H; auto.
 Qed.
 
-Lemma no_alias_head_tail_update :
-  forall pinfo ptr EC1 EC2 ECs
+Lemma no_alias_head_in_tail_update :
+  forall pinfo ombs EC1 EC2 
   (EQ: Opsem.CurFunction EC1 = Opsem.CurFunction EC2)
-  (Hp: forall gvsa (EQ': Opsem.CurFunction EC1 = PI_f pinfo)
-   (Hlkup: lookupAL (GVsT DGVs) (Opsem.Locals EC2) (PI_id pinfo) = ret gvsa),
-   lookupAL (GVsT DGVs) (Opsem.Locals EC1) (PI_id pinfo) = ret gvsa)
-  (Hnalias: no_alias_head_tail pinfo ptr (EC1 :: ECs)),
-  no_alias_head_tail pinfo ptr (EC2 :: ECs).
+  (Hp: forall (EQ': Opsem.CurFunction EC1 = PI_f pinfo),
+   lookupAL (GVsT DGVs) (Opsem.Locals EC2) (PI_id pinfo) =
+     lookupAL (GVsT DGVs) (Opsem.Locals EC1) (PI_id pinfo))
+  (Hnalias: no_alias_head_in_tail pinfo ombs EC1),
+  no_alias_head_in_tail pinfo ombs EC2.
+Proof.
+  intros.
+  unfold no_alias_head_in_tail in *.
+  intros. 
+  destruct Hnalias as [Hnalias1 Hnalias2].
+  split; intros.
+    rewrite Hp; try congruence.
+    apply Hnalias1; try solve [auto | congruence].
+
+    apply Hnalias2; try solve [auto | congruence].
+Qed.
+
+Lemma no_alias_head_tail_update :
+  forall pinfo ombs EC1 EC2 ECs
+  (EQ: Opsem.CurFunction EC1 = Opsem.CurFunction EC2)
+  (Hp: forall (EQ': Opsem.CurFunction EC1 = PI_f pinfo),
+   lookupAL (GVsT DGVs) (Opsem.Locals EC2) (PI_id pinfo) =
+     lookupAL (GVsT DGVs) (Opsem.Locals EC1) (PI_id pinfo))
+  (Hnalias: no_alias_head_tail pinfo ombs (EC1 :: ECs)),
+  no_alias_head_tail pinfo ombs (EC2 :: ECs).
 Proof.
   intros.
   unfold no_alias_head_tail in *.
-  intros.
-  simpl in Hin.
-  destruct Hin as [Hin | Hin]; subst.
-    assert (no_alias_head_in_tail pinfo ptr EC1) as J.
-      apply Hnalias; simpl; auto.
-    clear Hnalias.
-    unfold no_alias_head_in_tail in *. simpl in *. intros.
-    rewrite Heq in EQ.
-    apply J; auto.
-
-    apply Hnalias; simpl; auto.
+  inv Hnalias.
+  constructor; auto.
+    eapply no_alias_head_in_tail_update; eauto.
 Qed.
 
 Lemma switchToNewBasicBlock_sim : forall TD l1 l2 ps cs1 cs2 tmn1 tmn2 B1 B2
@@ -380,18 +388,22 @@ Admitted.
 Lemma mem_simulation_update_locals :
   forall pinfo TD EC1 EC2 ECs M1 M2
   (EQ: Opsem.CurFunction EC1 = Opsem.CurFunction EC2)
-  (Hp: forall gvsa
-   (Hlkup: lookupAL (GVsT DGVs) (Opsem.Locals EC1) (PI_id pinfo) = ret gvsa),
-   lookupAL (GVsT DGVs) (Opsem.Locals EC2) (PI_id pinfo) = ret gvsa)
-  (Hmsim: Mem_simulation pinfo TD (EC1 :: ECs) M1 M2),
-  Mem_simulation pinfo TD (EC2 :: ECs) M1 M2.
+  (Hp: forall (EQ': Opsem.CurFunction EC1 = PI_f pinfo),
+    lookupAL (GVsT DGVs) (Opsem.Locals EC1) (PI_id pinfo) =
+      lookupAL (GVsT DGVs) (Opsem.Locals EC2) (PI_id pinfo))
+  (Hmsim: mem_simulation pinfo TD (EC1 :: ECs) M1 M2),
+  mem_simulation pinfo TD (EC2 :: ECs) M1 M2.
 Proof.
   intros.
-  destruct Hmsim as [Hmsim1 Hmsim2].
+  destruct Hmsim as [Hmsim1 [Hmsim3 Hmsim2]].
   split; auto.
-    intros.
-    eapply Hmsim2 with (ptr:=ptr)(ty:=ty)(al:=al); eauto.
-    eapply no_alias_head_tail_update in Hnalias; eauto; simpl; auto.
+  split; auto.
+    unfold dse_mem_inj in *.
+    inv_mbind. clear HeqR.
+    intros ombs Hin.
+    apply Hmsim2. clear Hmsim2.
+    eapply no_alias_head_tail_update in Hin; eauto.
+      intros. apply Hp. congruence.
 Qed.
 
 Ltac destruct_ctx_other :=
@@ -419,7 +431,7 @@ match goal with
   destruct Hwfcfg as [_ [Hwfg [HwfSystem HmInS]]]; subst;
   destruct Hwfpp as
     [_ [
-     [Hreach1 [HBinF1 [HFinPs1 _]]]
+     [Hreach1 [HBinF1 [HFinPs1 [Hwflc1 _]]]]
      [ _ HwfCall'
      ]]
     ]; subst;
@@ -441,12 +453,38 @@ match goal with
   fold Promotability.wf_ECStack in HwfECs'
 end.
 
-Lemma mstore_palloca_Mem_simulation: forall TD M1 mp2 gv1 a M1' pinfo lc2 gl2
-  B1 cs1 tmn2 als2 ECs1 M2 i0 t v
-  (H23: mstore TD M1 mp2 t gv1 a = ret M1')
-  (H20: @Opsem.getOperandValue DGVs TD (value_id (PI_id pinfo)) lc2 gl2 =
+Lemma no_alias_head_in_tail_inv1: forall lc2 pinfo TD mb B1 cs1 tmn2 als2 y
+  (Hlkup: lookupAL (GVsT DGVs) lc2 (PI_id pinfo) =
+        ret ($ blk2GV TD mb # typ_pointer (PI_typ pinfo) $)) 
+  (H1 : no_alias_head_in_tail pinfo y
+         {|
+         Opsem.CurFunction := PI_f pinfo;
+         Opsem.CurBB := B1;
+         Opsem.CurCmds := cs1;
+         Opsem.Terminator := tmn2;
+         Opsem.Locals := lc2;
+         Opsem.Allocas := als2 |}),
+  y = ret mb.
+Proof.
+  intros.
+  destruct H1 as [H1 _]. simpl in H1.
+  rewrite Hlkup in H1.
+  rewrite Promotability.simpl_blk2GV in H1. tauto.
+Qed.
+
+Lemma mstore_palloca_mem_simulation: forall los nts M1 mp2 gv1 a M1' pinfo lc2 
+  gl2 B1 cs1 tmn2 als2 ECs1 M2 i0 t v maxb Ps S
+  (H23: mstore (los, nts) M1 mp2 t gv1 a = ret M1')
+  (H20: @Opsem.getOperandValue DGVs (los, nts) (value_id (PI_id pinfo)) lc2 gl2 =
           ret mp2)
-  (Hmsim: Mem_simulation pinfo TD
+  (Hinscope' : if fdef_dec (PI_f pinfo) (PI_f pinfo)
+              then Promotability.wf_defs maxb pinfo (los, nts) M1 lc2 als2
+              else True)
+  (H19 : Opsem.getOperandValue (los,nts) v lc2 gl2 = ret gv1)
+  (Hwfg : wf_global (los, nts) S gl2)
+  (Hwflc1 : OpsemPP.wf_lc (los, nts) (PI_f pinfo) lc2)
+  (Hwfv : wf_value S (module_intro los nts Ps) (PI_f pinfo) v t)
+  (Hmsim: mem_simulation pinfo (los, nts)
             ({|
              Opsem.CurFunction := PI_f pinfo;
              Opsem.CurBB := B1;
@@ -455,7 +493,7 @@ Lemma mstore_palloca_Mem_simulation: forall TD M1 mp2 gv1 a M1' pinfo lc2 gl2
              Opsem.Terminator := tmn2;
              Opsem.Locals := lc2;
              Opsem.Allocas := als2 |} :: ECs1) M1 M2),
-  Mem_simulation pinfo TD
+  mem_simulation pinfo (los, nts)
             ({|
              Opsem.CurFunction := PI_f pinfo;
              Opsem.CurBB := B1;
@@ -465,32 +503,54 @@ Lemma mstore_palloca_Mem_simulation: forall TD M1 mp2 gv1 a M1' pinfo lc2 gl2
              Opsem.Allocas := als2 |} :: ECs1) M1' M2.
 Proof.
   intros.
-  destruct Hmsim as [Hmsim1 Hmsim2].
+  destruct Hmsim as [Hmsim1 [Hmsim3 Hmsim2]].
   split.
     apply MemProps.nextblock_mstore in H23.
     rewrite <- H23. auto.
-
-    intros.
-    eapply Hmsim2; eauto using no_alias_head_tail_irrel.
-    eapply MemProps.mstore_preserves_mload_inv'; eauto.
-    assert (no_alias_head_in_tail pinfo ptr
-              {| Opsem.CurFunction := PI_f pinfo;
-                 Opsem.CurBB := B1;
-                 Opsem.CurCmds := cs1;
-                 Opsem.Terminator := tmn2;
-                 Opsem.Locals := lc2;
-                 Opsem.Allocas := als2 |}) as J.
-      apply Hnalias; simpl; auto.
-    apply MemProps.no_alias_sym.
-    unfold no_alias_head_in_tail in J; eauto.
+  split.
+    intro b'.    
+    eapply MemProps.bounds_mstore in H23; eauto.
+    rewrite <- H23. eauto.
+    
+    unfold dse_mem_inj in *. inv_mbind.
+    intros ombs Hin.
+    inv Hin.
+    assert (no_alias_head_tail pinfo (y::l')
+             ({|
+              Opsem.CurFunction := PI_f pinfo;
+              Opsem.CurBB := B1;
+              Opsem.CurCmds := insn_store i0 t v (value_id (PI_id pinfo)) a
+                               :: cs1;
+              Opsem.Terminator := tmn2;
+              Opsem.Locals := lc2;
+              Opsem.Allocas := als2 |} :: ECs1)) as Hin.
+      constructor; auto.     
+    apply Hmsim2 in Hin. clear Hmsim2.
+    simpl in Hin.
+    assert (t = PI_typ pinfo) as EQ.
+      admit. (* by wf *)
+    subst. simpl in H20.
+    assert (exists mb, mp2 = 
+              ($ (blk2GV (los,nts) mb) # (typ_pointer (PI_typ pinfo)) $)) as EQ.
+      destruct (fdef_dec (PI_f pinfo) (PI_f pinfo)); try congruence.
+      apply Hinscope' in H20.
+      destruct H20 as [[_ [[mb [H20 _]] _]] _]. eauto.
+    destruct EQ as [mb EQ]; subst.
+    assert (y = Some mb) as EQ.
+      eapply no_alias_head_in_tail_inv1; eauto.
+    subst.
+    assert (n = sizeGenericValue gv1) as EQ.
+      eapply wf__getTypeStoreSize_eq_sizeGenericValue; eauto.
+    subst.
+    simpl.
+    eapply SASmsim.mstore_inside_inj_left'; eauto.
 Qed.
 
 Ltac repeat_solve :=
   repeat (match goal with
-          | |- Mem_simulation _ _ _ _ _ => idtac
+          | |- mem_simulation _ _ _ _ _ => idtac
           | |- _ => split; eauto 2 using cmds_at_block_tail_next
           end).
-
 
 Lemma products_simulation__fdef_simulation : forall pinfo Ps1 Ps2 fid f1 f2,
   lookupFdefViaIDFromProducts Ps2 fid = Some f2 ->
@@ -539,7 +599,7 @@ Lemma lookupExFdecViaPtr__simulation_l2r : forall pinfo Ps1 Ps2 fptr f fs,
   OpsemAux.lookupExFdecViaPtr Ps1 fs fptr = Some f ->
   OpsemAux.lookupExFdecViaPtr Ps2 fs fptr = Some f.
 Admitted.
-
+(*
 Lemma no_alias_head_tail_cons_and: forall pinfo ptr EC ECs,
   no_alias_head_tail pinfo ptr (EC :: ECs) ->
   no_alias_head_in_tail pinfo ptr EC /\ no_alias_head_tail pinfo ptr ECs.
@@ -550,22 +610,22 @@ Proof.
     apply H; simpl; auto.
     intros. apply H; simpl; auto.
 Qed.
-
-Lemma callExternalFunction__Mem_simulation: forall pinfo TD St1 M1 M2 fid0 gvss0
+*)
+Lemma callExternalFunction__mem_simulation: forall pinfo TD St1 M1 M2 fid0 gvss0
   oresult1 M1' oresult2 M2' dck tr1 tr2 gl tret targs,
-  Mem_simulation pinfo TD St1 M1 M2 ->
+  mem_simulation pinfo TD St1 M1 M2 ->
   callExternalOrIntrinsics TD gl M1 fid0 tret targs dck gvss0 =
     ret (oresult1, tr1, M1') ->
   callExternalOrIntrinsics TD gl M2 fid0 tret targs dck gvss0 =
     ret (oresult2, tr2, M2') ->
-  oresult1 = oresult2 /\ Mem_simulation pinfo TD St1 M1' M2' /\ tr1 = tr2.
+  oresult1 = oresult2 /\ mem_simulation pinfo TD St1 M1' M2' /\ tr1 = tr2.
 Admitted.
 
 Ltac dse_is_sim_common_case :=
 match goal with
 | Hcssim2: cmds_simulation _ _ _ _,
   Hop2: Opsem.sInsn _ _ _ _,
-  Hmsim: Mem_simulation _ _ _ _ _ |- _ =>
+  Hmsim: mem_simulation _ _ _ _ _ |- _ =>
   apply cmds_simulation_nelim_cons_inv in Hcssim2; simpl; auto;
   destruct Hcssim2 as [cs3' [Heq Hcssim2]]; subst;
   inv Hop2; uniq_result;
@@ -574,14 +634,782 @@ match goal with
       eauto |
       simpl; intros;
       match goal with
-      | Hlkup : lookupAL _ ?lc ?id1 = Some ?gvsa |-
-        lookupAL _ (updateAddAL _ ?lc _ _ ) ?id1 = Some ?gvsa =>
+      | |- lookupAL _ ?lc ?id1 =
+             lookupAL _ (updateAddAL _ ?lc _ _ ) ?id1 =>
         admit  (* id <> palloca *)
       end]
 end.
 
+Lemma no_alias_head_tail__replace_head: forall EC' EC ECs1 ombs pinfo
+  (Hp : forall omb,
+        no_alias_head_in_tail pinfo omb EC' ->
+        no_alias_head_in_tail pinfo omb EC)
+  (H1: no_alias_head_tail pinfo ombs (EC' :: ECs1)),
+  no_alias_head_tail pinfo ombs (EC :: ECs1).
+Proof.
+  intros. inv H1. constructor; auto.
+Qed.
+
+Lemma mem_simulation__replace_head: forall TD ECs1 pinfo EC EC'
+  (Hp : forall omb : monad mblock,
+        no_alias_head_in_tail pinfo omb EC' ->
+        no_alias_head_in_tail pinfo omb EC) M1 M2
+  (Hmsim : mem_simulation pinfo TD (EC :: ECs1) M1 M2),
+  mem_simulation pinfo TD (EC' :: ECs1) M1 M2.
+Proof.
+  intros.
+  destruct Hmsim as [J1 [J2 J3]].
+  split; auto.
+  split; auto.
+    unfold dse_mem_inj in *.
+    inv_mbind.
+    intros ombs Hin'.
+    eapply no_alias_head_tail__replace_head in Hin'; eauto.
+Qed.
+
+Lemma mem_simulation__malloc: forall (pinfo : PhiInfo)
+  (tmn2 : terminator) (lc2 : Opsem.GVsMap) (als2 als2': list mblock)
+  (M2 : mem) (los : layouts) (nts : namedts) (F : fdef) (B : block) c align0
+  (EC : list Opsem.ExecutionContext) t id0 (Hid: getCmdID c = Some id0)
+  (cs : list cmd) (Mem : mem) (gn : GenericValue) (Mem' : mem) (mb : mblock)
+  (Heq3 : exists l1 : l,
+           exists ps1 : phinodes,
+             exists cs11 : list cmd,
+               B =
+               block_intro l1 ps1 (cs11 ++ c :: cs)
+                 tmn2)
+  (Hmalloc: match c with
+            | insn_malloc _ _ _ _ | insn_alloca _ _ _ _ => True
+            | _ => False
+            end) (Hwfpi: WF_PhiInfo pinfo)
+  (Hexeq: exists l1 : l, exists ps1 : phinodes,exists cs11 : list cmd,
+              B = block_intro l1 ps1 (cs11 ++ c :: cs) tmn2)
+  (HBinF: blockInFdefB B F = true) (Huniq: uniqFdef F)
+  (Hpalloca : palloca_props.wf_State pinfo
+                ({| Opsem.ECS := {|
+                         Opsem.CurFunction := F;
+                         Opsem.CurBB := B;
+                         Opsem.CurCmds := c :: cs;
+                         Opsem.Terminator := tmn2;
+                         Opsem.Locals := lc2;
+                         Opsem.Allocas := als2 |} :: EC;
+                    Opsem.Mem := Mem |}))
+  (Hmsim : mem_simulation pinfo (los, nts)
+            ({|
+             Opsem.CurFunction := F;
+             Opsem.CurBB := B;
+             Opsem.CurCmds := c :: cs;
+             Opsem.Terminator := tmn2;
+             Opsem.Locals := lc2;
+             Opsem.Allocas := als2 |} :: EC) Mem M2)
+  (Hnrem : ~
+          removable_State pinfo 
+            {|
+            Opsem.ECS := {|
+                         Opsem.CurFunction := F;
+                         Opsem.CurBB := B;
+                         Opsem.CurCmds := c :: cs;
+                         Opsem.Terminator := tmn2;
+                         Opsem.Locals := lc2;
+                         Opsem.Allocas := als2 |} :: EC;
+            Opsem.Mem := Mem |})
+  (Mem'0 : mem) (tsz0 : sz)
+  (H2 : malloc (los, nts) Mem tsz0 gn align0 = ret (Mem', mb))
+  (H25 : malloc (los, nts) M2 tsz0 gn align0 = ret (Mem'0, mb)),
+  mem_simulation pinfo (los, nts)
+     ({|
+      Opsem.CurFunction := F;
+      Opsem.CurBB := B;
+      Opsem.CurCmds := cs;
+      Opsem.Terminator := tmn2;
+      Opsem.Locals := updateAddAL (GVsT DGVs) lc2 id0
+                        ($ blk2GV (los, nts) mb # typ_pointer t $);
+      Opsem.Allocas := als2' |} :: EC) Mem' Mem'0.
+Proof.
+  intros.
+    destruct Hmsim as [Hmsim1 [Hmim3 Hmsim2]].
+    split.
+      apply MemProps.nextblock_malloc in H2.
+      apply MemProps.nextblock_malloc in H25.
+      rewrite <- H2. rewrite <- H25. rewrite Hmsim1. auto.
+    split.  
+      apply MemProps.bounds_malloc in H2.
+      apply MemProps.bounds_malloc in H25.
+      destruct H2 as [n [H21 H22]].
+      destruct H25 as [n' [H25 H26]].
+      rewrite H21 in H25. inv H25.
+      intro b.
+      rewrite H26. rewrite H22.
+      destruct (eq_block b mb); auto.
+
+      unfold dse_mem_inj in *.
+      inv_mbind. clear HeqR.
+      intros ombs Hin'. 
+      apply malloc_inv in H2. destruct H2 as [n0 [J1 [J2 J3]]].
+      apply malloc_inv in H25. destruct H25 as [n0' [J1' [J2' J3']]].
+      rewrite J1 in J1'. inv J1'.
+      eapply SASmsim.alloc_inject_id_inj with (m1:=Mem)(m2:=M2); eauto.
+      assert (ret getCmdLoc c = getCmdID c) as G.
+        erewrite getCmdLoc_getCmdID; eauto.
+      destruct (id_dec id0 (PI_id pinfo)); subst.
+        destruct c; tinv Hmalloc; simpl in *; inv Hid.
+          admit. (* malloc <> pid *)
+
+          inv Hin'.
+          assert (no_alias_head_tail pinfo (None::l')
+             ({|
+              Opsem.CurFunction := F;
+              Opsem.CurBB := B;
+              Opsem.CurCmds := insn_alloca (PI_id pinfo) t0 v a :: cs;
+              Opsem.Terminator := tmn2;
+              Opsem.Locals := lc2;
+              Opsem.Allocas := als2 |} :: EC)) as Hin.
+            unfold no_alias_head_tail.
+            constructor; auto.
+              split; simpl; intros; auto.
+                subst.
+                assert (lookupAL (GVsT DGVs) lc2 (PI_id pinfo) = None) as Hnone.
+                  clear - Hpalloca Hwfpi HBinF Huniq Hexeq.
+                  eapply WF_PhiInfo_spec15 in Hpalloca; eauto.
+                rewrite Hnone. auto.
+           apply_clear Hmsim2 in Hin.
+           simpl in Hin. 
+           simpl.
+           destruct y; auto.
+             simpl_env.
+             apply SASmsim.mem_inj_ignores_weaken; auto.
+
+        apply Hmsim2.
+        eapply no_alias_head_tail__replace_head in Hin'; eauto.
+        intros.
+        eapply no_alias_head_in_tail_update in H; eauto.
+          simpl. 
+          rewrite <- lookupAL_updateAddAL_neq; auto.
+Qed.
+
+Lemma mem_simulation__free : forall TD Mem1 Mem2 Mem1' Mem2'
+  ECs1 pinfo EC EC' ptr
+  (Hp: forall omb,
+       no_alias_head_in_tail pinfo omb EC' ->
+       no_alias_head_in_tail pinfo omb EC)
+  (Hmsim : mem_simulation pinfo TD (EC :: ECs1) Mem1 Mem2)
+  (Hmlc: free TD Mem1 ptr = ret Mem1')
+  (Hmlc': free TD Mem2 ptr = ret Mem2'),
+  mem_simulation pinfo TD (EC' :: ECs1) Mem1' Mem2'.
+Proof.
+  intros.
+  destruct Hmsim as [J1 [J2 J3]].
+  apply free_inv in Hmlc.
+  apply free_inv in Hmlc'.
+  destruct Hmlc as [blk [ofs [hi [lo [H1 [H2 [H3 H4]]]]]]].
+  destruct Hmlc' as [blk' [ofs' [hi' [lo' [H1' [H2' [H3' H4']]]]]]].
+  unfold GV2ptr in *.
+  destruct ptr as [|[[]][]]; inv H1. inv H1'.
+  split.
+    apply Mem.nextblock_free in H4'.
+    apply Mem.nextblock_free in H4. 
+    congruence.
+  split.
+    intros.
+    apply Mem.bounds_free with (b:=b) in H4'; auto.
+    apply Mem.bounds_free with (b:=b) in H4; auto.
+    congruence.
+
+    unfold dse_mem_inj in *.
+    inv_mbind.
+    intros ombs Hin'.
+    assert (no_alias_head_tail pinfo ombs (EC :: ECs1)) as Hin.
+      inv Hin'.
+      constructor; auto.
+    apply J3 in Hin.
+    eapply SASmsim.free_inj with (delta:=0)(b1:=blk')(b2:=blk') in Hin; 
+      eauto using SASmsim.inject_id_no_overlap, SASmsim.inject_id_zero_delta.
+    replace (lo+0) with lo by omega.
+    replace (hi+0) with hi by omega. 
+    rewrite J2 in H3. rewrite <- H3' in H3. inv H3. auto.
+Qed.
+
+Lemma mem_simulation__free_allocas : forall TD ECs1 pinfo EC EC'
+  (Hp: forall omb,
+       no_alias_head_in_tail pinfo omb EC' ->
+       no_alias_head_in_tail pinfo omb EC)
+  als Mem1 Mem2 Mem1' Mem2'
+  (Hmsim : mem_simulation pinfo TD (EC :: ECs1) Mem1 Mem2)
+  (Hmlc: free_allocas TD Mem1 als = ret Mem1')
+  (Hmlc': free_allocas TD Mem2 als = ret Mem2'),
+  mem_simulation pinfo TD (EC' :: ECs1) Mem1' Mem2'.
+Proof.
+  induction als; simpl; intros.
+    uniq_result. 
+    eapply mem_simulation__replace_head; eauto.
+
+    inv_mbind.
+    eapply mem_simulation__free with (Mem1':=m0)(Mem2':=m) in Hmsim; eauto.
+Qed.
+
+Lemma mem_simulation__remove_head: forall TD ECs1 pinfo EC 
+  (Hp : no_alias_head_in_tail pinfo None EC) M1 M2
+  (Hmsim : mem_simulation pinfo TD (EC :: ECs1) M1 M2),
+  mem_simulation pinfo TD ECs1 M1 M2.
+Proof.
+  intros.
+  destruct Hmsim as [J1 [J2 J3]].
+  split; auto.
+  split; auto.
+    unfold dse_mem_inj in *.
+    inv_mbind.
+    intros ombs Hin'.
+    replace (ombs__ignores (Size.to_Z n) ombs) with
+            (ombs__ignores (Size.to_Z n) (None::ombs)) by auto.
+    apply J3; auto.
+      constructor; auto.
+Qed.
+
+Lemma no_alias_head_in_tail_ex: forall pinfo EC,
+  exists omb, no_alias_head_in_tail pinfo omb EC.
+Proof.
+  unfold no_alias_head_in_tail.
+  intros. 
+  destruct (fdef_dec (Opsem.CurFunction EC) (PI_f pinfo)).
+    destruct (lookupAL (GVsT DGVs) (Opsem.Locals EC) (PI_id pinfo)) 
+      as [[|[[]][]]|]; eauto.
+      exists (Some b). tauto.
+
+    destruct (lookupAL (GVsT DGVs) (Opsem.Locals EC) (PI_id pinfo)) 
+      as [[|[[]][]]|]; eauto.
+      exists None. tauto.
+Qed.
+
+Lemma no_alias_head_tail_ex: forall pinfo ECs,
+  exists ombs, no_alias_head_tail pinfo ombs ECs.
+Proof.
+  unfold no_alias_head_tail.
+  induction ECs; simpl; eauto.
+    destruct IHECs as [ombs IHECs].
+    destruct (@no_alias_head_in_tail_ex pinfo a) as [omb J].
+    exists (omb::ombs). constructor; auto.
+Qed.
+
+Lemma no_alias_head_in_tail_inv3: forall lc2 pinfo mb B1 cs1 tmn2 als2 F
+  (H1 : no_alias_head_in_tail pinfo (Some mb)
+         {|
+         Opsem.CurFunction := F;
+         Opsem.CurBB := B1;
+         Opsem.CurCmds := cs1;
+         Opsem.Terminator := tmn2;
+         Opsem.Locals := lc2;
+         Opsem.Allocas := als2 |}),
+  F = PI_f pinfo /\
+  exists ofs, exists mc, 
+    lookupAL (GVsT DGVs) lc2 (PI_id pinfo) = ret ((Vptr mb ofs, mc)::nil).
+Proof.
+  intros.
+  destruct H1 as [H1 H2]. simpl in *.
+  destruct (fdef_dec F (PI_f pinfo)) as [J | J].
+    split; auto.
+      apply H1 in J.
+      destruct (lookupAL (GVsT DGVs) lc2 (PI_id pinfo)) 
+        as [[|[[]][]]|]; try solve [congruence | inv J; eauto].
+
+    apply H2 in J. congruence.
+Qed.
+
+Lemma mem_simulation__return: forall (pinfo : PhiInfo)
+  (lc2 : Opsem.GVsMap) (als2 : list mblock) (tmn3 : terminator) t0 v0 
+  (lc3 : Opsem.GVsMap) (als3 : list mblock) (M2 : mem) (los : layouts) 
+  (nts : namedts) (F : fdef) (rid : id) tmn (F' : fdef) (B' : block) (i0 : id)
+  (n : noret) (c : clattrs) (v : value) (p : params) (cs' : list cmd)
+  (EC : list Opsem.ExecutionContext) (Mem : mem) (l3 : l) (ps3 : phinodes)
+  (cs0 : list cmd) (Mem' : mem) (Hwfpi: WF_PhiInfo pinfo) Ps S
+  (HwfF: wf_fdef S (module_intro los nts Ps) F)
+  (H0 : free_allocas (los, nts) Mem als2 = ret Mem') maxb
+  (Heq3' : exists l1 : l,
+            exists ps1 : phinodes,
+              exists cs11 : list cmd,
+                B' =
+                block_intro l1 ps1 (cs11 ++ insn_call i0 n c t0 v0 v p :: cs')
+                  tmn3)
+  (Hinscope: if fdef_dec (PI_f pinfo) F
+             then Promotability.wf_defs maxb pinfo (los,nts) Mem lc2 als2
+             else True)
+  (Hmsim : mem_simulation pinfo (los, nts)
+            ({|
+             Opsem.CurFunction := F;
+             Opsem.CurBB := block_intro l3 ps3 (cs0 ++ nil) tmn;
+             Opsem.CurCmds := nil;
+             Opsem.Terminator := tmn;
+             Opsem.Locals := lc2;
+             Opsem.Allocas := als2 |}
+             :: {|
+                Opsem.CurFunction := F';
+                Opsem.CurBB := B';
+                Opsem.CurCmds := insn_call i0 n c t0 v0 v p :: cs';
+                Opsem.Terminator := tmn3;
+                Opsem.Locals := lc3;
+                Opsem.Allocas := als3 |} :: EC) Mem M2)
+  (Mem'0 : mem) (lc''0 : Opsem.GVsMap)
+  (EQ: lookupAL (GVsT DGVs) lc3 (PI_id pinfo) =
+         lookupAL (GVsT DGVs) lc''0 (PI_id pinfo))
+  (H26 : free_allocas (los, nts) M2 als2 = ret Mem'0),
+  mem_simulation pinfo (los, nts)
+     ({|
+      Opsem.CurFunction := F';
+      Opsem.CurBB := B';
+      Opsem.CurCmds := cs';
+      Opsem.Terminator := tmn3;
+      Opsem.Locals := lc''0;
+      Opsem.Allocas := als3 |} :: EC) Mem' Mem'0.
+Proof.
+  intros.
+  eapply mem_simulation__free_allocas in Hmsim; eauto.
+  destruct Hmsim as [Hmsim1 [Hmsim2 Hmsim3]].
+  split; auto.
+  split; auto.
+    unfold dse_mem_inj in *.
+    inv_mbind.
+    intros ombs Hin.
+    destruct (@no_alias_head_in_tail_ex pinfo 
+                {| Opsem.CurFunction := F;
+                   Opsem.CurBB := block_intro l3 ps3 (cs0 ++ nil) tmn;
+                   Opsem.CurCmds := nil;
+                   Opsem.Terminator := tmn;
+                   Opsem.Locals := lc2;
+                   Opsem.Allocas := als2 |}) as [omb G].
+    assert (no_alias_head_tail pinfo (omb::ombs)
+             ({|
+              Opsem.CurFunction := F;
+              Opsem.CurBB := block_intro l3 ps3 (cs0 ++ nil) tmn;
+              Opsem.CurCmds := nil;
+              Opsem.Terminator := tmn;
+              Opsem.Locals := lc2;
+              Opsem.Allocas := als2 |}
+              :: {|
+                 Opsem.CurFunction := F';
+                 Opsem.CurBB := B';
+                 Opsem.CurCmds := insn_call i0 n c t0 v0 v p :: cs';
+                 Opsem.Terminator := tmn3;
+                 Opsem.Locals := lc3;
+                 Opsem.Allocas := als3 |} :: EC)) as Hin'.
+      unfold no_alias_head_tail. unfold no_alias_head_tail in Hin.
+      constructor; auto.
+        inv Hin.
+        constructor; auto.
+          eapply no_alias_head_in_tail_update in H2; eauto.
+    apply_clear Hmsim3 in Hin'.
+      destruct omb as [mb|]; auto.
+      
+      simpl in Hin'.
+      apply SASmsim.mem_inj__remove_unperm_igns in Hin'; auto.
+      apply no_alias_head_in_tail_inv3 in G.
+      destruct G as [EQ1 [ofs [mc G]]]; subst.
+      destruct (fdef_dec (PI_f pinfo) (PI_f pinfo)); try congruence.
+      apply Hinscope in G.
+      destruct G as [[_ [[mb0 [G1 [G2 [G3 G4]]]] _]] _]; subst.
+      rewrite Promotability.simpl_blk2GV in G1. inv G1.
+      intros.
+      unfold Promotability.alloca_size_prop in G4.
+      unfold getTypeAllocSize in G4.
+      rewrite <- HeqR in G4.
+      remember (getABITypeAlignment (los, nts) (PI_typ pinfo)) as R.
+      destruct R; tinv G4.
+      remember (Mem.bounds Mem mb0) as R.
+      destruct R as [lo hi].
+      destruct (@G4 lo hi) as [G41 G42]; subst; auto.
+      eapply MemProps.perm_mfree_alloca_2 in H0; eauto.
+      assert (RoundUpAlignment n0 n1 >= n0)%nat as G.
+        apply RoundUpAlignment_spec.
+          eapply WF_PhiInfo_spec16 in HwfF; eauto.
+          unfold getABITypeAlignment, getAlignment in HeqR0.
+          destruct HwfF as [sz [al [J1 [J2 J3]]]].
+          rewrite J1 in HeqR0. inv HeqR0. auto.
+      unfold Size.to_Z in *.
+      omega.
+Qed. 
+
+Lemma no_alias_head_in_tail__wf_ECStack_head_in_tail__no_alias_with_blk: forall
+  (pinfo : PhiInfo) (lc2 : AssocList (GVsT DGVs))
+  (gv2 : GVsT DGVs) S los nts Ps (Mem : Mem.mem) F t v gl
+  (Hwfv: wf_value S (module_intro los nts Ps) F v t)
+  (maxb : Values.block) (Hget : getOperandValue (los,nts) v lc2 gl = ret gv2)
+  (EC : Opsem.ExecutionContext) (mb : mblock)
+  (H : no_alias_head_in_tail pinfo (ret mb) EC)
+  (Hwfg: MemProps.wf_globals maxb gl)
+  (Hnals1 : 
+    Promotability.wf_ECStack_head_in_tail maxb pinfo (los,nts) Mem lc2 EC),
+  MemProps.no_alias_with_blk gv2 mb.
+Proof.
+  intros.
+  unfold no_alias_head_in_tail in H.  
+  destruct H as [H1 H2]. 
+  destruct (fdef_dec (Opsem.CurFunction EC) (PI_f pinfo)) as [J | J].
+    assert (G:=J).
+    apply_clear H1 in J; auto.
+    remember (lookupAL (GVsT DGVs) (Opsem.Locals EC) (PI_id pinfo)) as R.
+    destruct R as [[|[[]][]]|]; tinv J.
+    inv J. symmetry in HeqR.
+    eapply wf_ECStack_head_in_tail__no_alias_with_blk; eauto.
+    
+    apply_clear H2 in J. congruence.
+Qed.
+
+Lemma no_alias_head_tail__wf_ECStack_head_tail__no_alias_with_blk: 
+  forall pinfo lc2 gv2 los nts Mem maxb size Ps F t gl
+  (Hwfg: MemProps.wf_globals maxb gl) v S
+  (Hwfv: wf_value S (module_intro los nts Ps) F v t)
+  (Hget : getOperandValue (los,nts) v lc2 gl = ret gv2) EC ombs
+  (Hdse: no_alias_head_tail pinfo ombs EC)
+  (Hnals: Promotability.wf_ECStack_head_tail maxb pinfo (los,nts) Mem lc2 EC),
+  List.Forall (fun re => 
+               let '(mb,_,_) := re in
+               MemProps.no_alias_with_blk gv2 mb) (ombs__ignores size ombs).
+Proof.
+  intros.
+  induction Hdse; simpl; intros; auto.
+    apply Promotability.wf_ECStack_head_tail_cons__inv in Hnals.
+    destruct Hnals as [Hnals1 Hals2].
+    apply_clear IHHdse in Hals2.
+    destruct y as [mb|]; auto.
+    constructor; auto.
+    eapply no_alias_head_in_tail__wf_ECStack_head_in_tail__no_alias_with_blk; 
+      eauto.
+Qed.
+
+Lemma no_alias_head_tail__notin_ignores_with_size': forall maxb pinfo  
+  los nts Mem lc2 EC gl
+  (Hnals: Promotability.wf_ECStack_head_tail maxb pinfo (los,nts) Mem lc2 EC)
+  (Hwfg: MemProps.wf_globals maxb gl) S Ps t v F 
+  (Hwfv: wf_value S (module_intro los nts Ps) F v (typ_pointer t))
+  b' ofs' m'
+  (Hget: getOperandValue (los,nts) v lc2 gl = Some ((Vptr b' ofs', m')::nil)) ombs size'
+  (Hin: no_alias_head_tail pinfo ombs EC) size,
+  SASmsim.notin_ignores_with_size (ombs__ignores size' ombs) b'
+     (Int.signed 31 ofs') size.
+Proof.
+  intros.
+  eapply no_alias_head_tail__wf_ECStack_head_tail__no_alias_with_blk 
+    with (size:=size') in Hin; eauto.
+  eapply SASmsim.no_alias_with_blk__notin_ignores_with_size; eauto.
+Qed.   
+
+Lemma no_alias_head_in_tail_dec: forall pinfo EC mb
+  (Hnone: no_alias_head_in_tail pinfo None EC)
+  (Hsome: no_alias_head_in_tail pinfo (Some mb) EC),
+  False.
+Proof.
+  unfold no_alias_head_in_tail.
+  intros.
+  destruct (fdef_dec (Opsem.CurFunction EC) (PI_f pinfo)) as [J | J].
+    assert (J':=J).
+    apply Hnone in J. 
+    apply Hsome in J'. 
+    destruct (lookupAL (GVsT DGVs) (Opsem.Locals EC) (PI_id pinfo)) 
+      as [[|[[]][]]|]; inv J; inv J'.
+
+    assert (J':=J).
+    apply Hnone in J. 
+    apply Hsome in J'. 
+    destruct (lookupAL (GVsT DGVs) (Opsem.Locals EC) (PI_id pinfo)) 
+      as [[|[[]][]]|]; inv J; inv J'.
+Qed.
+
+Lemma unused_pid_no_alias_head_in_tail__wf_defs__no_alias_with_blk: 
+  forall pinfo F los nts maxb Mem lc2 EC gv2 als2
+  (Hinscope: if fdef_dec (PI_f pinfo) F
+             then Promotability.wf_defs maxb pinfo (los,nts) Mem lc2 als2
+             else True)
+  gl (Hwfg: MemProps.wf_globals maxb gl) v S t Ps
+  (Hwfv: wf_value S (module_intro los nts Ps) F v t)
+  (Hget : getOperandValue (los,nts) v lc2 gl = ret gv2) mb
+  (Hneq: used_in_value (PI_id pinfo) v = false)
+  (Heq1: Opsem.CurFunction EC = F) (Heq2: Opsem.Locals EC = lc2)
+  (Heq3: Opsem.Allocas EC = als2)
+  (Hdse: no_alias_head_in_tail pinfo (Some mb) EC),
+  MemProps.no_alias_with_blk gv2 mb.
+Proof.
+  intros.
+  destruct Hdse as [J1 J2]. subst.
+  destruct (fdef_dec (PI_f pinfo) (Opsem.CurFunction EC)) as [J | J].
+    symmetry in J. assert (G:=J).
+    apply_clear J1 in J.
+    remember (lookupAL (GVsT DGVs) (Opsem.Locals EC) (PI_id pinfo)) as R.
+    destruct R as [[|[[]][]]|]; inv J.
+    clear J2. symmetry in HeqR.
+    eapply wf_defs__no_alias_with_blk; eauto.
+
+    assert (Opsem.CurFunction EC <> PI_f pinfo) as G. intro K. auto.
+    apply J2 in G. congruence.
+Qed.
+
+Lemma no_alias_head_in_tail_inv2: forall EC pinfo y
+  (Heq : Opsem.CurFunction EC <> PI_f pinfo)
+  (H1 : no_alias_head_in_tail pinfo y EC), y = None.
+Proof.
+  intros.
+  destruct H1 as [_ H1]. auto.
+Qed.
+
+Lemma load_notin_cmds__unused_in_value: forall vid0 id0 t v align0 cs cs11,
+  load_in_cmds vid0 (cs11 ++ insn_load id0 t v align0 :: cs) = false ->
+  used_in_value vid0 v = false.
+Proof. 
+  unfold load_in_cmds. intros.
+  remember false as R. rewrite HeqR in H at 2. rewrite HeqR. clear HeqR.
+  generalize dependent R. 
+  induction cs11; simpl; intros; eauto.
+    apply fold_left_eq in H.
+      apply orb_false_iff in H.
+      destruct H; auto.
+
+      intros a b J.
+      apply orb_false_iff in J.
+      destruct J; auto.
+Qed.
+
+Lemma load_notin_fdef__unused_in_value: forall F v t id0 align0 cs B tmn2 vid0
+  (Hnld: load_in_fdef vid0 F = false) (HBinF: blockInFdefB B F = true)
+  (Heq3 : exists l1 : l,
+           exists ps1 : phinodes,
+             exists cs11 : list cmd,
+               B =
+               block_intro l1 ps1
+                 (cs11 ++ insn_load id0 t v align0 :: cs) tmn2),
+  used_in_value vid0 v = false.
+Proof.
+  destruct F as [fh bs]. simpl. intros.
+  remember false as R. rewrite HeqR in Hnld at 2. rewrite HeqR. clear HeqR.
+  generalize dependent R. 
+  induction bs; simpl in *; intros.
+    inv HBinF.
+
+    apply orb_true_iff in HBinF.
+    destruct HBinF as [HBinF | HBinF]; eauto 2.
+      apply blockEqB_inv in HBinF.
+      subst.
+
+      clear IHbs.
+      apply fold_left_eq in Hnld.
+        apply orb_false_iff in Hnld.
+        destruct Hnld.
+        destruct Heq3 as [l1 [ps1 [cs11 Heq3]]]; subst.
+        simpl in H0.
+        apply load_notin_cmds__unused_in_value in H0; auto.
+
+        intros c b J.
+        apply orb_false_iff in J.
+        destruct J; auto.
+Qed.
+
+Lemma no_alias_head_tail__notin_ignores_with_size: forall maxb pinfo
+  los nts Mem lc2 EC gl
+  (Hnals: Promotability.wf_ECStack_head_tail maxb pinfo (los,nts) Mem lc2 EC)
+  (Hwfg: MemProps.wf_globals maxb gl) S Ps als2 tmn2 id0 t align0 v cs B F
+  (Hwfv: wf_value S (module_intro los nts Ps) F v (typ_pointer t))
+  (Hinscope: if fdef_dec (PI_f pinfo) F
+             then Promotability.wf_defs maxb pinfo (los,nts) Mem lc2 als2
+             else True) b' ofs' m'
+  (Hget: getOperandValue (los,nts) v lc2 gl = Some ((Vptr b' ofs', m')::nil)) ombs size'
+  (Hnld: load_in_fdef (PI_id pinfo) (PI_f pinfo) = false)
+  (HBinF: blockInFdefB B F = true)
+  (Heq3 : exists l1 : l,
+           exists ps1 : phinodes,
+             exists cs11 : list cmd,
+               B =
+               block_intro l1 ps1
+                 (cs11 ++ insn_load id0 t v align0 :: cs) tmn2)
+  (Hin: no_alias_head_tail pinfo ombs 
+        ({|
+         Opsem.CurFunction := F;
+         Opsem.CurBB := B;
+         Opsem.CurCmds := insn_load id0 t v align0 :: cs;
+         Opsem.Terminator := tmn2;
+         Opsem.Locals := lc2;
+         Opsem.Allocas := als2 |} :: EC)) size,
+  SASmsim.notin_ignores_with_size (ombs__ignores size' ombs) b'
+     (Int.signed 31 ofs') size.
+Proof.
+  intros.
+  inv Hin. simpl.
+  eapply no_alias_head_tail__notin_ignores_with_size' with (size:=size)(size':=size') 
+    in H3; eauto.
+  destruct y as [mb|]; auto.
+    unfold SASmsim.notin_ignores_with_size in *.
+    constructor; auto.
+    remember (used_in_value (PI_id pinfo) v) as R.
+    destruct R.
+      destruct (fdef_dec F (PI_f pinfo)); subst.
+        eapply load_notin_fdef__unused_in_value in Hnld; eauto.
+        congruence.
+
+        apply no_alias_head_in_tail_inv2 in H1; simpl; auto. congruence.
+      
+      eapply unused_pid_no_alias_head_in_tail__wf_defs__no_alias_with_blk in H1; 
+        eauto.
+      simpl in H1. auto.
+Qed.
+
+Lemma mem_simulation__mload: forall (maxb : Z) (pinfo : PhiInfo) 
+  (gl2 : GVMap) (fs2 : GVMap) (tmn2 : terminator)
+  (lc2 : Opsem.GVsMap) (als2 : list mblock) (M2 : mem) (S : system)
+  (los : layouts) (nts : namedts) (Ps : list product) (F : fdef) (B : block)
+  (id0 : id) (t : typ) (align0 : align) (v : value)
+  (EC : list Opsem.ExecutionContext) (cs : list cmd) (Mem : mem)
+  (mp : GenericValue) (gv : GenericValue)
+  (H1 : mload (los, nts) Mem mp t align0 = ret gv)
+  (Hwfg : MemProps.wf_globals maxb gl2)
+  (Hnld: load_in_fdef (PI_id pinfo) (PI_f pinfo) = false)
+  (HBinF: blockInFdefB B F = true)
+  (Heq3 : exists l1 : l,
+           exists ps1 : phinodes,
+             exists cs11 : list cmd,
+               B =
+               block_intro l1 ps1
+                 (cs11 ++ insn_load id0 t v align0 :: cs) tmn2)
+  (Hmsim : mem_simulation pinfo (los, nts)
+            ({|
+             Opsem.CurFunction := F;
+             Opsem.CurBB := B;
+             Opsem.CurCmds := insn_load id0 t v align0 :: cs;
+             Opsem.Terminator := tmn2;
+             Opsem.Locals := lc2;
+             Opsem.Allocas := als2 |} :: EC) Mem M2)
+  (Hinscope' : if fdef_dec (PI_f pinfo) F
+              then Promotability.wf_defs maxb pinfo (los, nts) Mem lc2 als2
+              else True)
+  (HwfHT : Promotability.wf_ECStack_head_tail maxb pinfo (los, nts) Mem lc2 EC)
+  (gv0 : GenericValue) (H23 : mload (los, nts) M2 mp t align0 = ret gv0)
+  (H21 : Opsem.getOperandValue (los, nts) v lc2 gl2 = ret mp)
+  (Hwfv : wf_value S (module_intro los nts Ps) F v (typ_pointer t)),
+  gv = gv0.
+Proof.
+  intros.
+  destruct Hmsim as [Hmsim1 [Hmsim3 Hmsim2]].
+  simpl in HwfHT.
+  apply mload_inv in H1.
+  destruct H1 as [b [ofs [m [mc [J1 [J2 J3]]]]]]; subst.
+  apply mload_inv in H23.
+  destruct H23 as [b' [ofs' [m' [mc' [J1' [J2' J3']]]]]]; subst.
+  rewrite J2 in J2'. inv J2'. inv J1'.
+  unfold dse_mem_inj in Hmsim2.
+  inv_mbind. clear HeqR.
+  destruct (@no_alias_head_tail_ex pinfo 
+             ({| Opsem.CurFunction := F;
+                 Opsem.CurBB := B;
+                 Opsem.CurCmds := insn_load id0 t v align0 :: cs;
+                 Opsem.Terminator := tmn2;
+                 Opsem.Locals := lc2;
+                 Opsem.Allocas := als2 |} :: EC)) as [ombs Hin].
+  assert (G:=Hin).
+  apply_clear Hmsim2 in Hin.
+  eapply SASmsim.mload_aux_inject_id_inj2; eauto.
+    eapply no_alias_head_tail__notin_ignores_with_size; eauto.
+Qed.
+
+Lemma mstore_unremovable_mem_simulation: forall (maxb : Z) (pinfo : PhiInfo)
+  (gl2 : GVMap) (tmn2 : terminator) 
+  (lc2 : Opsem.GVsMap) (als2 : list mblock) (M2 : mem) (S : system)
+  (los : layouts) (nts : namedts) (Ps : list product) (F : fdef) (B : block)
+  (sid : id) (t : typ) (align0 : align) (v1 : value) (v2 : value)
+  (EC : list Opsem.ExecutionContext) (cs : list cmd) (Mem : mem)
+  (HBinF1 : blockInFdefB B F = true) (mp2 : GenericValue) (gv1 : GenericValue)
+  (Mem' : mem) (H3 : mstore (los, nts) Mem mp2 t gv1 align0 = ret Mem')
+  (Hwfg : wf_global (los, nts) S gl2) (Hwflc1 : OpsemPP.wf_lc (los, nts) F lc2)
+  (Heq3 : exists l1 : l,
+           exists ps1 : phinodes,
+             exists cs11 : list cmd,
+               B =
+               block_intro l1 ps1
+                 (cs11 ++ insn_store sid t v1 v2 align0 :: cs) tmn2)
+  (Hmsim : mem_simulation pinfo (los, nts)
+            ({|
+             Opsem.CurFunction := F;
+             Opsem.CurBB := B;
+             Opsem.CurCmds := insn_store sid t v1 v2 align0 :: cs;
+             Opsem.Terminator := tmn2;
+             Opsem.Locals := lc2;
+             Opsem.Allocas := als2 |} :: EC) Mem M2)
+  (Hnrem : ~
+          removable_State pinfo 
+            {|
+            Opsem.ECS := {|
+                         Opsem.CurFunction := F;
+                         Opsem.CurBB := B;
+                         Opsem.CurCmds := insn_store sid t v1 v2 align0 :: cs;
+                         Opsem.Terminator := tmn2;
+                         Opsem.Locals := lc2;
+                         Opsem.Allocas := als2 |} :: EC;
+            Opsem.Mem := Mem |})
+  (Hinscope' : if fdef_dec (PI_f pinfo) F
+              then Promotability.wf_defs maxb pinfo (los, nts) Mem lc2 als2
+              else True)
+  (Mem'0 : mem)
+  (H24 : Opsem.getOperandValue (los, nts) v1 lc2 gl2 = ret gv1)
+  (H25 : Opsem.getOperandValue (los, nts) v2 lc2 gl2 = ret mp2)
+  (H28 : mstore (los, nts) M2 mp2 t gv1 align0 = ret Mem'0)
+  (Hwfv : wf_value S (module_intro los nts Ps) F v1 t),
+  mem_simulation pinfo (los, nts)
+     ({|
+      Opsem.CurFunction := F;
+      Opsem.CurBB := B;
+      Opsem.CurCmds := cs;
+      Opsem.Terminator := tmn2;
+      Opsem.Locals := lc2;
+      Opsem.Allocas := als2 |} :: EC) Mem' Mem'0.
+Proof.
+  intros.
+  destruct Hmsim as [Hmsim1 [Hmsim3 Hmsim2]].
+  split.
+    apply MemProps.nextblock_mstore in H3.
+    apply MemProps.nextblock_mstore in H28.
+    rewrite <- H3. rewrite <- H28. rewrite Hmsim1. auto.
+  
+  split.
+    intro b.
+    apply MemProps.bounds_mstore with (b':=b) in H3.
+    apply MemProps.bounds_mstore with (b':=b) in H28.
+    congruence.
+  
+    apply mstore_inversion in H28.
+    destruct H28 as [b [ofs [cm [J1 J2]]]]; subst.
+    apply mstore_inversion in H3.
+    destruct H3 as [b' [ofs' [cm' [J1' J2']]]]; subst.
+    inv J1'.
+    unfold dse_mem_inj in *.
+    inv_mbind.
+    intros ombs Hin'.
+    eapply no_alias_head_tail_irrel in Hin'.
+    eapply_clear Hmsim2 in Hin'.
+    eapply SASmsim.mstore_aux_inject_id_mapped_inj2; eauto.
+Qed.
+
+Ltac dse_is_sim_malloc :=
+  destruct_ctx_other;
+  match goal with 
+  | Hcssim2: cmds_simulation _ _ _ _,
+    Hop2: Opsem.sInsn _ _ _ _ |- _ =>
+    apply cmds_simulation_nelim_cons_inv in Hcssim2; simpl; auto;
+    destruct Hcssim2 as [cs3' [Heq Hcssim2]]; subst;
+    inv Hop2; uniq_result
+  end;
+  match goal with
+  | Hmsim: mem_simulation _ _ _ ?M1 ?M2,
+    H25: malloc _ ?M1 _ _ _ = Some (_, ?mb),
+    H2: malloc _ ?M2 _ _ _ = Some (_, ?mb0) |- _ =>
+    assert (mb0 = mb) as EQ; try solve [
+      match goal with
+      | |- _ = _ =>
+        destruct Hmsim as [Hmsim _];
+        apply MemProps.malloc_result in H25;
+        apply MemProps.malloc_result in H2; subst; auto
+      end
+    ]
+  end;
+  subst;
+  repeat_solve;
+    eapply mem_simulation__malloc; eauto using wf_system__uniqFdef; simpl; auto.
+
 Lemma dse_is_sim : forall maxb pinfo Cfg1 St1 Cfg2 St2
   (Hwfpi: WF_PhiInfo pinfo)
+  (Hwfmg: MemProps.wf_globals maxb (OpsemAux.Globals Cfg1)) 
   (Hnld: load_in_fdef (PI_id pinfo) (PI_f pinfo) = false)
   (Hwfcfg: OpsemPP.wf_Config Cfg1) (Hwfpp: OpsemPP.wf_State Cfg1 St1)
   (Hnoalias: Promotability.wf_State maxb pinfo Cfg1 St1)
@@ -614,7 +1442,7 @@ Case "removable state".
   destruct Hwfcfg as [_ [Hwfg [HwfSystem HmInS]]].
   destruct Hwfpp as
     [_ [
-     [Hreach1 [HBinF1 [HFinPs1 _]]]
+     [Hreach1 [HBinF1 [HFinPs1 [Hwflc1 _]]]]
      [HwfECs Hwfcall]]
     ]; subst.
   fold (@OpsemPP.wf_ECStack DGVs) in HwfECs.
@@ -643,7 +1471,9 @@ Case "removable state".
   uniq_result.
   repeat_solve.
     eapply cmds_simulation_elim_cons_inv; eauto.
-    eapply mstore_palloca_Mem_simulation in Hmsim; eauto.
+    assert (wf_value S1 (module_intro los nts Ps1) (PI_f pinfo) v t) as Hwfv.
+      admit. (* wf *)
+    eapply mstore_palloca_mem_simulation in Hmsim; eauto.
 
 Case "unremovable state".
   (sInsn_cases (destruct Hop1) SCase).
@@ -652,51 +1482,21 @@ SCase "sReturn".
 Focus.
   destruct_ctx_return.
   repeat_solve.
-
-    clear - H26 Hmsim H0 H1 Hinscope1' HBinF2 Heq3'.
-    destruct Hmsim as [Hmsim1 Hmsim2].
-    split.
-      apply MemProps.nextblock_free_allocas in H0.
-      apply MemProps.nextblock_free_allocas in H26.
-      rewrite <- H0. rewrite <- H26. auto.
-
-      intros.
-      eapply Hmsim2 with (ptr:=ptr)(ty:=ty)(al:=al);
-        eauto using MemProps.free_allocas_preserves_mload_inv.
-      clear Hmsim2.
-      apply no_alias_head_tail_and_cons; simpl.
-        eapply no_alias_head_in_tail__return; eauto.
-
-        unfold Opsem.returnUpdateLocals in H1.
-        inv_mbind'.
-        destruct n; inv H2.
-          eapply no_alias_head_tail_irrel; eauto.
-          inv_mbind'.
-          eapply no_alias_head_tail_update in Hnalias; eauto; simpl; auto.
-          intros.
-          destruct (id_dec i0 (PI_id pinfo)); subst.
-            admit. (* callid <> palloca *)
-            rewrite <- lookupAL_updateAddAL_neq; auto.
+    assert (wf_fdef S (module_intro los nts Ps) F) as HwfF.
+      eauto using wf_system__wf_fdef.
+    clear - H26 Hmsim H0 H1 Heq3' Hinscope1' HwfF Hwfpi.
+    eapply mem_simulation__return; eauto.
+      admit. (* pid <> i0 *)
 Unfocus.
 
 SCase "sReturnVoid".
 Focus.
   destruct_ctx_return.
   repeat_solve.
-
-    clear - H24 Hmsim H0 Hinscope1'.
-    destruct Hmsim as [Hmsim1 Hmsim2].
-    split.
-      apply MemProps.nextblock_free_allocas in H0.
-      apply MemProps.nextblock_free_allocas in H24.
-      rewrite <- H0. rewrite <- H24. auto.
-
-      intros.
-      eapply Hmsim2 with (ptr:=ptr)(ty:=ty)(al:=al);
-        eauto using MemProps.free_allocas_preserves_mload_inv.
-      apply no_alias_head_tail_and_cons; simpl.
-        eapply no_alias_head_in_tail__return; eauto.
-        eapply no_alias_head_tail_irrel; eauto.
+    assert (wf_fdef S (module_intro los nts Ps) F) as HwfF.
+      eauto using wf_system__wf_fdef.
+    clear - H24 Hmsim H0 Heq3' Hinscope1' HwfF Hwfpi.
+    eapply mem_simulation__return; eauto.
 Unfocus.
 
 SCase "sBranch".
@@ -763,43 +1563,7 @@ SCase "sBop". abstract (destruct_ctx_other; dse_is_sim_common_case).
 SCase "sFBop". abstract (destruct_ctx_other; dse_is_sim_common_case).
 SCase "sExtractValue". abstract (destruct_ctx_other; dse_is_sim_common_case).
 SCase "sInsertValue". abstract (destruct_ctx_other; dse_is_sim_common_case).
-SCase "sMalloc".
-
-  destruct_ctx_other.
-
-  apply cmds_simulation_nelim_cons_inv in Hcssim2; simpl; auto;
-  destruct Hcssim2 as [cs3' [Heq Hcssim2]]; subst;
-  inv Hop2; uniq_result.
-
-  assert (mb0 = mb) as EQ.
-    destruct Hmsim as [Hmsim _].
-    apply MemProps.malloc_result in H25.
-    apply MemProps.malloc_result in H2. subst. auto.
-  subst.
-  repeat_solve.
-
-    destruct Hmsim as [Hmsim1 Hmsim2].
-    split; auto.
-      apply MemProps.nextblock_malloc in H2.
-      apply MemProps.nextblock_malloc in H25.
-      rewrite <- H2. rewrite <- H25. rewrite Hmsim1. auto.
-
-      intros.
-      eapply MemProps.malloc_preserves_mload_inv in Hld1; eauto.
-      eapply MemProps.malloc_preserves_mload_inv in Hld2; eauto.
-      destruct (@MemProps.no_alias_with_blk_dec mb ptr) 
-        as [Halias_mb | Hnalias_mb].
-        destruct Hld1 as [[Hld1 _]|[_ G]]; try congruence.
-        destruct Hld2 as [[Hld2 _]|[_ G]]; try congruence.
-        eapply no_alias_head_tail_update in Hnalias; eauto; simpl; auto.
-          intros. admit. (* id <> palloca *)
-        
-        destruct Hld1 as [[_ G]|[Hld1 _]]; try congruence.
-        destruct Hld2 as [[_ G]|[Hld2 _]]; try congruence.
-        (* two cases, if ptr is mb or not,
-           malloc_preserves_mload_inv needs to be extended to match chunks!. *)
-        admit.
-
+SCase "sMalloc". abstract (dse_is_sim_malloc).
 SCase "sFree".
 
   destruct_ctx_other.
@@ -809,78 +1573,27 @@ SCase "sFree".
   inv Hop2; uniq_result.
 
   repeat_solve.
-    destruct Hmsim as [Hmsim1 Hmsim2].
-    split; auto.
-      apply MemProps.nextblock_free in H1.
-      apply MemProps.nextblock_free in H22.
-      rewrite <- H1. rewrite <- H22. rewrite Hmsim1. auto.
+    eapply mem_simulation__free; eauto.
+    eapply mem_simulation__replace_head in Hmsim; eauto.
 
-      intros.
-      eapply Hmsim2 with (ptr:=ptr)(ty:=ty)(al:=al);
-        eauto using MemProps.free_preserves_mload_inv.
-      eapply no_alias_head_tail_irrel in Hnalias; eauto; simpl; auto.
-
-SCase "sAlloca".
-
-  destruct_ctx_other.
-
-  apply cmds_simulation_nelim_cons_inv in Hcssim2; simpl; auto;
-  destruct Hcssim2 as [cs3' [Heq Hcssim2]]; subst;
-  inv Hop2; uniq_result.
-
-  assert (mb0 = mb) as EQ.
-    destruct Hmsim as [Hmsim _].
-    apply MemProps.malloc_result in H25.
-    apply MemProps.malloc_result in H2. subst. auto.
-  subst.
-  repeat_solve.
-
-    destruct Hmsim as [Hmsim1 Hmsim2].
-    split; auto.
-      apply MemProps.nextblock_malloc in H2.
-      apply MemProps.nextblock_malloc in H25.
-      rewrite <- H2. rewrite <- H25. rewrite Hmsim1. auto.
-
-      intros.
-      eapply MemProps.malloc_preserves_mload_inv in Hld1; eauto.
-      eapply MemProps.malloc_preserves_mload_inv in Hld2; eauto.
-      destruct (@MemProps.no_alias_with_blk_dec mb ptr) 
-        as [Halias_mb | Hnalias_mb].
-        destruct Hld1 as [[Hld1 _]|[_ G]]; try congruence.
-        destruct Hld2 as [[Hld2 _]|[_ G]]; try congruence.
-        eapply no_alias_head_tail_update in Hnalias; eauto; simpl; auto.
-        destruct (id_dec id0 (PI_id pinfo)); subst.
-          intros gvsa Heq Hlkup; subst.
-          assert (uniqFdef (PI_f pinfo)) as Huniq.
-            eauto using wf_system__uniqFdef.
-          clear - Hlkup Hpalloca HBinF1 Heq3 Huniq Hwfpi.
-          assert (lookupAL (GVsT DGVs) lc2 (PI_id pinfo) = None) as Hnone.
-            eapply WF_PhiInfo_spec15; eauto.
-          congruence.
-
-          intros.
-          rewrite <- lookupAL_updateAddAL_neq; auto.
-        
-        destruct Hld1 as [[_ G]|[Hld1 _]]; try congruence.
-        destruct Hld2 as [[_ G]|[Hld2 _]]; try congruence.
-        (* two cases, if ptr is mb or not,
-           malloc_preserves_mload_inv needs to be extended to match chunks!. *)
-        admit.
+SCase "sAlloca". abstract (dse_is_sim_malloc).
 
 SCase "sLoad".
   destruct_ctx_other.
 
-  apply cmds_simulation_nelim_cons_inv in Hcssim2; simpl; auto;
+  apply cmds_simulation_nelim_cons_inv in Hcssim2; simpl; auto.
   destruct Hcssim2 as [cs3' [Heq Hcssim2]]; subst;
   inv Hop2; uniq_result.
 
   assert (gv = gv0) as EQ.
-    admit. (* no load from pid *)
+    assert (wf_value S (module_intro los nts Ps) F v (typ_pointer t)) as Hwfv.
+      admit. (* wf *)
+    clear - H23 Hmsim H1 H21 HwfHT Hinscope' Hwfmg Hwfv Heq3 Hnld HBinF1. 
+    simpl in *.
+    eapply mem_simulation__mload; eauto.
   subst.
   repeat_solve.
-
     eapply mem_simulation_update_locals in Hmsim; simpl; eauto.
-      simpl. intros.
       admit. (* lid <> pid *)
 
 SCase "sStore".
@@ -898,22 +1611,15 @@ SCase "sStore".
     destruct (id_dec i0 (PI_id pinfo)); subst; auto.
     destruct (id_dec (PI_id pinfo) (PI_id pinfo)); try congruence.
     contradict Hnrem; auto.
-  apply cmds_simulation_nelim_cons_inv in Hcssim2; auto.
+  apply cmds_simulation_nelim_cons_inv in Hcssim2; simpl; auto.
   destruct Hcssim2 as [cs3' [Heq Hcssim2]]; subst;
   inv Hop2; uniq_result.
 
   repeat_solve.
-    destruct Hmsim as [Hmsim1 Hmsim2].
-    split; auto.
-      apply MemProps.nextblock_mstore in H3.
-      apply MemProps.nextblock_mstore in H28.
-      rewrite <- H3. rewrite <- H28. rewrite Hmsim1. auto.
-
-      intros.
-      eapply Hmsim2 with (ptr:=ptr)(ty:=ty)(al:=al); eauto.
-      eapply no_alias_head_tail_irrel in Hnalias; eauto; simpl; auto.
-        (* same to sas, we should use lower msim *)
-        admit. admit.
+    assert (wf_value S (module_intro los nts Ps) F v1 t) as Hwfv.
+      admit. (* wf *)
+    clear - Hwfv H28 H24 H3 Hwflc1 Heq3 Hmsim HBinF1 Hinscope' H25 Hwfg Hnrem.
+    eapply mstore_unremovable_mem_simulation; eauto.
 
 SCase "sGEP". abstract (destruct_ctx_other; dse_is_sim_common_case).
 SCase "sTrunc". abstract (destruct_ctx_other; dse_is_sim_common_case).
@@ -965,13 +1671,24 @@ SCase "sCall".
     destruct Hfsim1 as [Heq _]. inv Heq. uniq_result.
     auto.
 
-    destruct Hmsim as [Hmsim1 Hmsim2].
+    destruct Hmsim as [Hmsim1 [Hmsim3 Hmsim2]].
     split; auto.
-      intros.
-      eapply Hmsim2 with (ptr:=ptr)(ty:=ty)(al:=al); eauto.
-      clear Hmsim2.
-      apply no_alias_head_tail_cons_and in Hnalias.
-      destruct Hnalias as [Hnalias1 Hnalias2]; auto.
+    split; auto.
+       clear - Hmsim2 Hwfpi H4 H1 HwfSystem HmInS.
+       unfold dse_mem_inj in *.
+       inv_mbind. 
+       intros ombs Hin'.
+       inv Hin'.
+       assert (y = None) as EQ.
+         destruct (fdef_dec (fdef_intro (fheader_intro fa rt fid la va) lb) 
+                          (PI_f pinfo)).
+           apply OpsemAux.lookupFdefViaPtr_inv in H1; auto.
+           eapply arguments_dont_define_pid in H4; eauto using wf_system__uniqFdef.
+           destruct H2 as [H2 _]. simpl in H2.
+           apply H2 in e. rewrite H4 in e. auto.
+
+           apply no_alias_head_in_tail_inv2 in H2; simpl; auto.
+        subst. simpl. apply Hmsim2; auto.
 
   SSCase "sExCall".
 
@@ -1025,7 +1742,7 @@ SCase "sExCall".
   eapply lookupExFdecViaPtr__simulation_l2r in Hlkdec; eauto.
   uniq_result.
 
-  eapply callExternalFunction__Mem_simulation in Hmsim; eauto.
+  eapply callExternalFunction__mem_simulation in Hmsim; eauto.
   destruct Hmsim as [EQ [Hmsim EQ']]; subst.
   uniq_result.
   repeat_solve.
